theories/case_studies/iterator.v
@@ -9,8 +9,8 @@ From hazel.program_logic Require Import weakest_precondition
                                         state_reasoning.
 
 (* Local imports *)
-From haffel.lang Require Import haffel.
-From haffel.case_studies Require Import representable.
+From affect.lang Require Import affect.
+From affect.case_studies Require Import representable.
 
 
 Section iterator.
