theories/case_studies/promotion.v
@@ -1,0 +1,100 @@
+
+From stdpp Require Import base list.
+From iris.proofmode Require Import base tactics.
+From iris.algebra Require Import excl_auth.
+
+
+(* Hazel Reasoning *)
+From hazel.program_logic Require Import weakest_precondition 
+                                        tactics 
+                                        shallow_handler_reasoning 
+                                        deep_handler_reasoning 
+                                        state_reasoning.
+
+(* Local imports *)
+From affect.lib Require Import base.
+From affect.lang Require Import affect.
+From affect.logic Require Import sem_def.
+From affect.logic Require Import sem_env.
+From affect.logic Require Import sem_sig.
+From affect.logic Require Import sem_row.
+From affect.logic Require Import sem_types.
+From affect.logic Require Import sem_judgement.
+From affect.logic Require Import copyable.
+From affect.logic Require Import sem_operators.
+From affect.logic Require Import compatibility.
+From affect.logic Require Import tactics.
+
+(* Make all the definitions opaque so that we do not rely on their definition in the model to show that the programs are well-typed terms. *)
+Opaque sem_typed sem_typed_val ty_le row_le sig_le row_type_sub row_env_sub.
+Opaque sem_ty_void sem_ty_unit sem_ty_bool sem_ty_int sem_ty_string sem_ty_top sem_ty_cpy sem_env_cpy sem_ty_ref_cpy sem_ty_ref sem_ty_prod sem_ty_sum sem_ty_arr sem_ty_aarr sem_ty_uarr sem_ty_forall sem_ty_row_forall sem_ty_exists sem_ty_rec sem_ty_option sem_ty_list.
+Opaque sem_sig_eff sem_sig_os.
+Opaque sem_row_nil sem_row_os sem_row_tun sem_row_cons sem_row_rec.
+
+
+Definition mk_one_shot : val := (λ: <>, 
+    shandle[OS]: (perform: "op" #()) by 
+      "op" => (λ: "x" "k", "k")
+    | ret  => (λ: "x", (λ: "y", "y")) 
+    end)%V.
+
+  Definition mk_one_shot_dp : val := (λ: <>, 
+      let: "r" := ref (λ: <>, #()) in
+        handle[OS]: (perform: "op" #()) by
+        "op" => (λ: "x" "k", "r" <!- "k";; #())
+        | ret  => (λ: "x", "x")
+        end ;; "r" <!- (λ: <>, #())
+  )%V.
+
+Section typing.
+
+  Context `{!heapGS Σ}.
+
+  Definition op_eff : operation * sem_sig Σ := ("op", ∀S: (_ : sem_ty Σ), () =[OS]=> ())%S.
+  Definition op_row : sem_row Σ := (op_eff · ⟨⟩)%R.
+  Definition mk_os_ty : sem_ty Σ := (() → (() -{ op_row }-∘ ()))%T.
+  Definition mk_os_dp_ty : sem_ty Σ := (() → (() ⊸ ()))%T.
+
+  Lemma mk_one_shot_typed : 
+    ⊢ (⊨ᵥ mk_one_shot : mk_os_ty).
+  Proof.
+    iIntros. rewrite /mk_one_shot /mk_os_ty.
+    iApply sem_typed_closure; solve_sidecond. simpl.
+    iApply (sem_typed_shandler (TT:=[tele _]) OS "op" (tele_app (λ (_ : sem_ty Σ), ())) (tele_app (λ _, ())) () (() -{ op_row }-∘ ()) ⟨⟩%R ⟨⟩%R [] [] [] [] "x" "k" with "[] []"); solve_sidecond.
+    { iRight. solve_copy. }
+    { iApply row_le_refl. }
+    - iApply (sem_typed_perform_os (TT:=[tele _]) [tele_arg ()] with "[]"). 
+      iApply sem_typed_unit'.
+    - simpl. iIntros (?). iApply sem_typed_weaken.
+      rewrite -/op_eff -/op_row. iApply sem_typed_var. 
+    - simpl. iApply sem_typed_weaken. 
+      rewrite - {1} (app_nil_r []).
+      iApply sem_typed_afun; solve_sidecond. simpl.
+      iApply sem_typed_var'.
+  Qed.
+
+  Lemma mk_one_shot_typed_dp : 
+    ⊢ (⊨ᵥ mk_one_shot_dp : mk_os_dp_ty).
+  Proof.
+    iIntros. rewrite /mk_one_shot_dp /mk_os_ty.
+    iApply sem_typed_closure; solve_sidecond. simpl.
+    iApply (sem_typed_let (Refᶜ (() ⊸ ())) _ _ _ []); solve_sidecond.
+    { iApply sem_typed_alloc_cpy. 
+      rewrite - {1} (app_nil_r []). iApply sem_typed_afun; solve_sidecond. iApply sem_typed_unit. }
+    iApply sem_typed_contraction; solve_copy.
+    set r := ("r", Refᶜ (() ⊸ ())).
+    iApply (sem_typed_seq () _ _ _ [r]). iApply sem_typed_frame.
+    - replace [r] with ([] ++ [r]) by done.
+      iApply (sem_typed_handler (TT:=[tele _]) OS "op" (tele_app (λ (_ : sem_ty Σ), ())) (tele_app (λ _, ())) () () ⟨⟩%R ⟨⟩%R [] [] [] [r] "x" "k" with "[] []"); solve_sidecond.
+      + iApply row_le_refl.
+      + iApply (sem_typed_perform_os (TT:=[tele _]) [tele_arg ()] with "[]"). 
+        iApply sem_typed_unit'.
+      + simpl. iIntros (?). iApply sem_typed_weaken.
+        iApply (sem_typed_seq (() ⊸ ()) ⟨⟩%R () _ []); last iApply sem_typed_unit.
+        iApply sem_typed_replace_cpy_os; iApply sem_typed_var.
+      + simpl. iApply sem_typed_swap_second. iApply sem_typed_weaken.
+        iApply sem_typed_var.
+    - iApply sem_typed_replace_cpy_os; first iApply sem_typed_var.
+      replace [r] with ([] ++ [r]) by done.
+      iApply sem_typed_afun; solve_sidecond. simpl. iApply sem_typed_unit.
+  Qed.
