theories/case_studies/state.v
@@ -12,18 +12,18 @@ From hazel.program_logic Require Import weakest_precondition
                                         state_reasoning.
 
 (* Local imports *)
-From haffel.lib Require Import base.
-From haffel.lang Require Import haffel.
-From haffel.logic Require Import sem_def.
-From haffel.logic Require Import sem_env.
-From haffel.logic Require Import sem_sig.
-From haffel.logic Require Import sem_row.
-From haffel.logic Require Import sem_types.
-From haffel.logic Require Import sem_judgement.
-From haffel.logic Require Import copyable.
-From haffel.logic Require Import sem_operators.
-From haffel.logic Require Import compatibility.
-From haffel.logic Require Import tactics.
+From affect.lib Require Import base.
+From affect.lang Require Import affect.
+From affect.logic Require Import sem_def.
+From affect.logic Require Import sem_env.
+From affect.logic Require Import sem_sig.
+From affect.logic Require Import sem_row.
+From affect.logic Require Import sem_types.
+From affect.logic Require Import sem_judgement.
+From affect.logic Require Import copyable.
+From affect.logic Require Import sem_operators.
+From affect.logic Require Import compatibility.
+From affect.logic Require Import tactics.
 
 (* Make all the definitions opaque so that we do not rely on their definition in the model to show that the programs are well-typed terms. *)
 Opaque sem_typed sem_typed_val ty_le row_le sig_le row_type_sub row_env_sub.
