theories/lang/subst_map.v
@@ -6,7 +6,7 @@
 *)
 
 (* Local imports *)
-From haffel.lib Require Import base.
+From affect.lib Require Import base.
 
 Fixpoint subst_map (vs : gmap string val) (e : expr) : expr :=
   match e with
