theories/logic/ewpw.v
@@ -14,12 +14,12 @@ From hazel.program_logic Require Import weakest_precondition
                                         protocols.
 
 (* Local imports *)
-From haffel.lib Require Import logic.
-From haffel.lang Require Import haffel.
-From haffel.logic Require Import sem_def.
-From haffel.logic Require Import mode.
-From haffel.logic Require Import sem_sig.
-From haffel.logic Require Import sem_row.
+From affect.lib Require Import logic.
+From affect.lang Require Import affect.
+From affect.logic Require Import sem_def.
+From affect.logic Require Import mode.
+From affect.logic Require Import sem_sig.
+From affect.logic Require Import sem_row.
 
 (* EWP wrapper *)
 Definition ewpw `{!heapGS Σ} (E : coPset) (e : expr) (ρ : sem_row Σ) (Φ : val -d> iPropO Σ) : iPropO Σ := 
