theories/logic/mode.v
@@ -9,9 +9,9 @@ From hazel.program_logic Require Import weakest_precondition
                                         protocols.
 
 (* Local imports *)
-From haffel.lib Require Import logic.
-From haffel.lang Require Import haffel.
-From haffel.logic Require Import sem_def.
+From affect.lib Require Import logic.
+From affect.lang Require Import affect.
+From affect.logic Require Import sem_def.
 
 Definition mode_mult m m' : mode :=
   match m with
